dimsum_examples/compiler/linearize.v
@@ -219,18 +219,16 @@ Proof.
       move => /Hvsi'' [|[?|?]]; [ |set_unfold; naive_solver lia..].
       move => /Hvsi'; set_unfold; naive_solver lia.
   - move => /= ? IH ????????????????? Hcont. prepare_goal.
-    apply :IH; [done|done|done|set_solver|set_solver|done|].
+    apply: IH; [done|done|done|set_solver|set_solver|done|].
     intros ???????Hvsi' =>/=. erewrite lookup_var_val_to_expr; [|done].
     destruct v' eqn:?.
-    2,3: tstep_s; split!; intros; done.
+    2,3: tstep_s; split!; done.
     destruct (decide (z>0)) eqn:?.
-    2:{ tstep_s. split!; intros. inversion H4.
-        split; last first. intros; subst; done.
-        split!. apply heap_fresh_is_fresh.
+    2:{ tstep_s. split! => *; [apply heap_fresh_is_fresh|]. tstep_s => *; done. 
         Unshelve. all: apply inhabitant. }
-    tstep_i. intros. split; try done.
-    tstep_i. tstep_s. split!. intros. split!; [naive_solver|naive_solver|].
-    intros. rewrite -subst_subst_map_delete.
+    tstep_i => *. split; [done|]. destruct!.
+    tstep_i. tstep_s => *. split! => *; [done|].  
+    rewrite -subst_subst_map_delete.
     apply :tsim_mono_b. destruct!. apply: Hcont.
     + lia.
     + by simplify_map_eq.
